examples/rv/rv32.v
@@ -4,7 +4,7 @@ Require Import RV.RVCore.
 Import RV32ICore.
 
 Definition rv_schedule : scheduler :=
-    Writeback |> Execute |> Decode |> WaitImem |> Fetch |> ExternalI |> ExternalD  |> done.
+    MultiplierWriteback |> Writeback |> Execute |> StepMultiplier |> Decode |> WaitImem |> Fetch |> ExternalI |> ExternalD  |>  done.
 
 Definition circuits :=
   compile_scheduler rv_rules rv_external rv_schedule.
